trying to not reply on Lambda

Affine/Affine.lean
@@ -19,7 +19,7 @@ namespace Affine
 /-- The number of abstractions, useful for `termination_by` for normalization. -/
 def size (e : Affine vs) : ℕ :=
   match e with
-  | .var _ => 0
+  | .var _ => 1
   | .abs _ e => 1 + e.size
   | .app e₁ e₂ _ => e₁.size + e₂.size
 
